Made stack conversion deterministic again

02Stack/StackConversion.thy
@@ -2,86 +2,60 @@ theory StackConversion
 imports EvaluateStack
 begin
 
-inductive unstack :: "nat set \<Rightarrow> frame list \<Rightarrow> expr \<Rightarrow> expr heap \<Rightarrow> nat set \<Rightarrow> frame list \<Rightarrow> expr \<Rightarrow> 
-    bool" where
-  us_nil [simp]: "unstack xs [] e h xs [] e"
-| us_sref [simp]: "x \<notin> free_vars e \<Longrightarrow> unstack xs s (Var x) (update\<^sub>h h x e) xs' s' e' \<Longrightarrow> 
-    unstack xs (SRef x # s) e h xs' s' e'"
-| us_sapp [simp]: "unstack xs s (App e e\<^sub>2) h xs' s' e' \<Longrightarrow> unstack xs (SApp e\<^sub>2 # s) e h xs' s' e'"
-| us_sproj [simp]: "unstack xs s (Proj e l) h xs' s' e' \<Longrightarrow> unstack xs (SProj l # s) e h xs' s' e'"
-| us_scase [simp]: "unstack xs s (Case e t cs) h xs' s' e' \<Longrightarrow> 
-    unstack xs (SCase t cs # s) e h xs' s' e'"
-| us_sunfold [simp]: "unstack xs s (Unfold t e) h xs' s' e' \<Longrightarrow> 
-    unstack xs (SUnfold t # s) e h xs' s' e'"
-| us_styapp [simp]: "unstack xs s (TyApp e t) h xs' s' e' \<Longrightarrow> unstack xs (STyApp t # s) e h xs' s' e'"
-| us_let [simp]: "x \<notin> free_vars\<^sub>s\<^sub>s s \<Longrightarrow> x \<notin> xs \<Longrightarrow> 
-    x \<notin> \<Union> ((\<lambda>y. free_vars (lookup\<^sub>h y h)) ` {y. y < length\<^sub>h h \<and> y \<noteq> x \<and> y \<notin> xs}) \<Longrightarrow>
-      unstack (insert x xs) s (Let (lookup\<^sub>h x h) (incr\<^sub>e\<^sub>e x (subst\<^sub>x\<^sub>e x 0 e))) h xs' s' e' \<Longrightarrow> 
-        unstack xs s e h xs' s' e'"
+fun unfold_heap :: "nat list \<Rightarrow> expr heap \<Rightarrow> expr \<Rightarrow> expr" where
+  "unfold_heap r h e = foldr Let (map (\<lambda>x. lookup\<^sub>h x h) r) e"
 
-inductive unstack_state :: "stack_state \<Rightarrow> expr \<Rightarrow> bool" where
-  uss_eval [simp]: "unstack {} s e h {x. x < length\<^sub>h h} [] e' \<Longrightarrow> 
-    unstack_state (StackState (Eval e) s h) e'"
-| uss_return [simp]: "unstack {} s (devalue v) h {x. x < length\<^sub>h h} [] e' \<Longrightarrow> 
-    unstack_state (StackState (Return v) s h) e'"
+fun unstack :: "nat list list \<Rightarrow> frame list \<Rightarrow> expr \<Rightarrow> expr heap \<Rightarrow> expr" where
+  "unstack [] s e h = undefined"
+| "unstack (r # rs) [] e h = unfold_heap r h e"
+| "unstack (r # rs) (SRef x # s) e h = unstack rs s (unfold_heap r h (Var x)) (update\<^sub>h h x e)"
+| "unstack (r # rs) (SApp e\<^sub>2 # s) e h = unstack rs s (unfold_heap r h (App e e\<^sub>2)) h"
+| "unstack (r # rs) (SProj l # s) e h = unstack rs s (unfold_heap r h (Proj e l)) h"
+| "unstack (r # rs) (SCase t cs # s) e h = unstack rs s (unfold_heap r h (Case e t cs)) h"
+| "unstack (r # rs) (SUnfold t # s) e h = unstack rs s (unfold_heap r h (Unfold t e)) h"
+| "unstack (r # rs) (STyApp t # s) e h = unstack rs s (unfold_heap r h (TyApp e t)) h"
 
-lemma tc_unstack [elim]: "unstack xs s e h {x. x < length\<^sub>h h} [] e' \<Longrightarrow> \<Gamma> \<turnstile>\<^sub>s\<^sub>s s : t \<rightarrow> t' \<Longrightarrow> 
-  [],\<Gamma> \<turnstile> e : t \<Longrightarrow> h \<turnstile>\<^sub>h \<Gamma> \<Longrightarrow> free_vars e \<inter> xs = {} \<Longrightarrow> free_vars\<^sub>s\<^sub>s s \<inter> xs = {} \<Longrightarrow> 
-    (\<forall>x \<in> xs. \<forall>y \<in> {x. x < length\<^sub>h h}. y \<notin> xs \<longrightarrow> x \<notin> free_vars (lookup\<^sub>h y h)) \<Longrightarrow> [],[] \<turnstile> e' : t'"
-  proof (induction xs s e h "{x. x < length\<^sub>h h}" "[] :: frame list" e' arbitrary: t
-         rule: unstack.induct)
-  case (us_nil e h)
-    hence L: "length\<^sub>h h = length \<Gamma>" by blast
-    from us_nil have "[],\<Gamma> \<turnstile> e : t'" by blast
-    moreover from us_nil L have "free_vars e \<inter> {x. x < length \<Gamma>} = {}" by simp
-    ultimately show ?case by simp
-  next case (us_sref xs s x h e e')
-    moreover hence "{x. x < length\<^sub>h h} = {xa. xa < length\<^sub>h (update\<^sub>h h x e)}"
-      by (metis length\<^sub>h_update\<^sub>h)
-    moreover from us_sref(3) have "[],\<Gamma> \<turnstile> Var x : t" by fastforce
-    moreover from us_sref(3, 4, 5) have "update\<^sub>h h x e \<turnstile>\<^sub>h \<Gamma>" by fastforce
-    moreover from us_sref(7) have "free_vars (Var x) \<inter> xs = {}" by fastforce
-    moreover from us_sref(7) have "free_vars\<^sub>s\<^sub>s s \<inter> xs = {}" by fastforce
-    moreover from us_sref(6, 8) have "\<forall>x' \<in> xs. \<forall>y \<in> {z. z < length\<^sub>h (update\<^sub>h h x e)}. y \<notin> xs \<longrightarrow> 
-      x' \<notin> free_vars (lookup\<^sub>h y (update\<^sub>h h x e))" by auto
-    ultimately show ?case by blast
-  next case us_sapp
+fun unstack_state :: "nat list list \<Rightarrow> stack_state \<Rightarrow> expr" where
+  "unstack_state rs (StackState (Eval e) s h) = unstack rs s e h"
+| "unstack_state rs (StackState (Return v) s h) = unstack rs s (devalue v) h"
+
+lemma tc_unstack [elim]: "\<Gamma> \<turnstile>\<^sub>s\<^sub>s s : t \<rightarrow> t' \<Longrightarrow> [],\<Gamma> \<turnstile> e : t \<Longrightarrow> h \<turnstile>\<^sub>h \<Gamma> \<Longrightarrow> 
+  distinct (concat rs) \<Longrightarrow> set (concat rs) = {x. x < length\<^sub>h h} \<Longrightarrow> length rs = Suc (length s) \<Longrightarrow>
+    [],[] \<turnstile> unstack rs s e h : t'"
+  proof (induction rs s e h rule: unstack.induct)
+  case 1
     thus ?case by simp
-  next case us_sproj
-    thus ?case by simp
-  next case us_scase
-    thus ?case by simp
-  next case us_sunfold
-    thus ?case by simp
-  next case us_styapp
-    thus ?case by simp
-  next case (us_let x s xs h e e')
-    from us_let(1) have "x \<notin> free_vars\<^sub>s\<^sub>s s" by simp
-    from us_let(2) have "x \<notin> xs" by simp
-    from us_let(3) have "x \<notin> \<Union>((\<lambda>y. free_vars (lookup\<^sub>h y h)) ` {y. y < length\<^sub>h h \<and> y \<noteq> x \<and> y \<notin> xs})" by simp
-    from us_let(4) have "unstack (insert x xs) s (expr.Let (lookup\<^sub>h x h) (incr\<^sub>e\<^sub>e x (subst\<^sub>x\<^sub>e x 0 e))) h {x. x < length\<^sub>h h} [] e'" by simp
-    from us_let(6) have "\<Gamma> \<turnstile>\<^sub>s\<^sub>s s : t \<rightarrow> t'" by simp
-    from us_let(7) have "[] ,\<Gamma> \<turnstile> e : t" by simp
-    from us_let(8) have "h \<turnstile>\<^sub>h \<Gamma>" by simp
-    from us_let(9) have "free_vars e \<inter> xs = {}" by simp
-    from us_let(10) have "free_vars\<^sub>s\<^sub>s s \<inter> xs = {}" by simp                 
-    from us_let(11) have "\<forall>x\<in>xs. \<forall>y\<in>{x. x < length\<^sub>h h}. y \<notin> xs \<longrightarrow> x \<notin> free_vars (lookup\<^sub>h y h)" by simp
+  next case (2 r rs e h)
+    hence "rs = []" by fastforce
+
+    from 2 have "\<Gamma> \<turnstile>\<^sub>s\<^sub>s [] : t \<rightarrow> t'" by simp
+    from 2 have "[] ,\<Gamma> \<turnstile> e : t" by simp
+    from 2 have "h \<turnstile>\<^sub>h \<Gamma>" by simp
+    from 2 have "distinct (concat (r # rs))" by simp
+    from 2 have "set (concat (r # rs)) = {x. x < length\<^sub>h h}" by simp
 
 
-    have A: "[],\<Gamma> \<turnstile> Let (lookup\<^sub>h x h) (incr\<^sub>e\<^sub>e x (subst\<^sub>x\<^sub>e x 0 e)) : t" by simp
-
-
-    have B: "free_vars (Let (lookup\<^sub>h x h) (incr\<^sub>e\<^sub>e x (subst\<^sub>x\<^sub>e x 0 e))) \<inter> insert x xs = {}" by simp
-    from us_let have "\<forall>xa\<in>insert x xs. \<forall>y\<in>{x. x < length\<^sub>h h}. y \<notin> insert x xs \<longrightarrow> 
-      xa \<notin> free_vars (lookup\<^sub>h y h)" by auto
-    with us_let A B show ?case by blast
+    have "[],[] \<turnstile> foldr Let (map (\<lambda>x. lookup\<^sub>h x h) r) e : t'" by simp
+    thus ?case by simp
+  next case 3
+    thus ?case by simp
+  next case 4
+    thus ?case by simp
+  next case 5
+    thus ?case by simp
+  next case 6
+    thus ?case by simp
+  next case 7
+    thus ?case by simp
+  next case 8
+    thus ?case by simp
   qed
 
-lemma tc_unstack_state [elim]: "unstack_state \<Sigma> e \<Longrightarrow> \<Sigma> hastype t \<Longrightarrow> [],[] \<turnstile> e : t"
-  proof (induction \<Sigma> e rule: unstack_state.induct)
-  case uss_eval
+lemma tc_unstack_state [elim]: "\<Sigma> hastype t \<Longrightarrow> [],[] \<turnstile> unstack_state rs \<Sigma> : t"
+  proof (induction rs \<Sigma> rule: unstack_state.induct)
+  case 1
     thus ?case using tc_unstack tc_eval_state by blast
-  next case uss_return
+  next case 2
     thus ?case using tc_unstack tc_return_state tc_devalue by blast
   qed
 
